\section{Bruchgesetze}
\begin{frame}
    \frametitle{Bruchgesetze}
	\begin{enumerate}
		\setlength\itemsep{1em}
		\item $\frac{a}{b}=\frac{ac}{bc}$
		\item $\frac{a}{b}=\frac{a \div c}{b \div c}$
		\item $\frac{a}{b}*c=\frac{ac}{b}$
		\item $\frac{a}{b}*c^{-1}=\frac{a}{bc}$
		\item $\frac{a}{b} \div c=\frac{a}{bc}$
	\end{enumerate}
\end{frame}

\begin{frame}
    \frametitle{Bruchgesetze Rechenarten}
	\begin{enumerate}
		\setlength\itemsep{1em}
		\item $\frac{a}{b} + \frac{c}{b}=\frac{a+c}{b}$
		\item $\frac{a}{b} - \frac{c}{b}=\frac{a-c}{b}$
		\item $\frac{a}{b} + \frac{c}{d}=\frac{ad+bc}{bd}$
		\item $\frac{a}{b} = \frac{1}{\frac{b}{a}}$
		\item $\frac{a}{b} \div \frac{c}{d} = \frac{\frac{a}{b}}{\frac{c}{d}} = \frac{ad}{bc}$
	\end{enumerate}
\end{frame}


\begin{frame}
    \frametitle{Binomische Formeln Übungen}
	\begin{enumerate}
		\setlength\itemsep{1em}
		\item $\frac{a}{b} * (1 - \frac{c}{1-c})$ 
		\item $\frac{a}{\ln(1)}$
		\item $\frac{6p + 11}{2p + 4} - \frac{2p + 5}{p^2 +2p} -3$
	\end{enumerate}
\end{frame}

\begin{frame}
    \frametitle{Binomische Formeln Übungen Lösungen}
	\begin{enumerate}
		\setlength\itemsep{1em}
		\item $\frac{a}{b} * (1 - \frac{c}{1-c}) = \frac{ac}{b(1-c)}$
		\item $\frac{a}{\ln(1)}$ Nicht erlaubt, da durch 0 geteilt wird
		\item $\frac{6p + 11}{2p + 4} - \frac{2p + 5}{p^2 +2p} -3 = -\frac{5}{2p}$
	\end{enumerate}
\end{frame}


