\section{Potenzgesetze}
\begin{frame}
    \frametitle{Potenzgesetze}
	\begin{itemize}
		\setlength\itemsep{1em}
		\item $a^m * a^n = a^{m+n}$
		\item $\frac{a^m}{a^n} = a^{m-n}$
		\item $a^n * b^n = (ab)^n$
		\item $\frac{a^n}{b^n} = \frac{a}{b}^n$
		\item $(a^m)^n = a^{m*n}$
		\item $a^0 = 1$
		\item $a^{-n} = \frac{1}{a^n}$
	\end{itemize}
\end{frame}

\begin{frame}
    \frametitle{Potenzgesetze Übungen}
	\begin{enumerate}
		\setlength\itemsep{1em}
		\item $\frac{1^3}{5^n}$
		\item $\frac{5^0- \sin(a^2) + \cos(a^2)}{\ln(e)}$
		\item $x^{-n} * x$
		\item $\frac{x^5 +1}{x^{m+2}} - \frac{2x^2-2}{x^m} + \frac{2-x}{x^{m-2}}$
	\end{enumerate}
\end{frame}

\begin{frame}
    \frametitle{Potenzgesetze Lösungen}
	\begin{enumerate}
		\setlength\itemsep{1em}
		\item $\frac{1^3}{5^n} = \frac{1}{5}^n$
		\item $\frac{5^0- \sin(a^2) + \cos(a^2)}{\ln(e)} = 1$
		\item $x^{-n} * x = x^{-n+1}$
		\item $\frac{1+2x^2}{x^{m+2}}$
	\end{enumerate}
\end{frame}

