\section{Vollständige Induktion}
\begin{frame}
    \frametitle{Vollständige Induktion}
    Zu beweisende Aussage: $\sum_{i=1}^{n} i = \frac{n(n+1)}{2}$
    \vfill
    \begin{itemize}
        \vfill \item Induktionsanfang(IA)($n=1$):
                \newline $\sum_{i=1}^{1} i = \frac{1(1+1)}{2} = 1$
        \vfill \item Induktionsvoraussetzung(IV):
                \newline Die Aussage gelte für ein beliebiges aber festes $n \in \mathbb{N}$
        \vfill \item Induktionsschritt(IS)($n \Rightarrow n+1$):
                \newline $\sum_{i=1}^{n+1} i = \sum_{i=1}^{n} i + (n+1) \stackrel{IV}{=} \frac{n(n+1)}{2} + (n+1) = \frac{n(n+1)}{2} + \frac{2n+2}{2} = \frac{n(n+1)+2n+2}{2} = \frac{(n+1)(n+2)}{2} \blacksquare$

    \end{itemize}
\end{frame}
